---
title:  最小二乘法推导
date: "2017-06-21"
author: 刘有才
---

#  OSL

一个简单的线性拟合如下：

```
plot(women$height, women$weight)
abline(lm(weight ~ height, data = women))
```

```{r echo=FALSE}
plot(women$height, women$weight)
fit <- lm(weight ~ height, data = women)
abline(fit)
# summary(fit)
segments(women$height, women$weight, women$height, fitted(fit), col = 2, lwd = 2)
legend("topleft", legend = "y=ax+b")
```

1. RSS

$$
\begin{cases}
y = ax +b \\ \\
RSS = \sum_{i=1}^n \big [y_i-(ax_i+b) \big ]^2
\end{cases}
$$

2. partial

$$
\begin{cases} 
\frac{\partial RSS}{\partial a} = -2 \sum x_i \big [y_i-(ax_i+b) \big] = 
-2 \big( \sum x_i y_i - a \sum x_i^2 - b \sum x_i \big)
\\ \\
\frac{\partial RSS}{\partial b} = -2 \sum \big [y_i-(ax_i+b) \big] = 
-2\big(\sum y_i -a \sum x_i - nb \big)
\end{cases}
$$

3. equation

$$
\begin{cases} 
\frac{\partial RSS}{\partial b} = 0 \\ \\
\sum y_i -a \sum x_i - nb = 0 \\ \\
n \overline{Y} - an \overline{X} - nb = 0 \\ \\
b = \overline{Y} - a \overline{X}
\end{cases}
$$

<p><p>

$$
\begin{cases}
\frac{\partial RSS}{\partial a} = 0 \\ \\
\sum x_i y_i - a \sum x_i^2 - b \sum x_i = 0 \\ \\
\sum x_i y_i - a \sum x_i^2 - \big( \overline{Y} - a \overline{X} \big) \sum x_i = 0 \\ \\
% \sum x_i y_i - a \sum x_i^2 - \overline{Y} \sum x_i  + a \overline{X} \sum x_i = 0 \\ \\
\sum x_i y_i  - \overline{Y} \sum x_i  = a \sum x_i^2 - a \overline{X} \sum x_i\\ \\
a = \frac{\sum x_iy_i - \overline{Y} \sum x_i} {\sum x_i^2 - \overline{X} \sum x_i} =
\frac{\sum \big(x_i-\overline{X}\big) \big(y_i-\overline{Y}\big)}{\sum \big(x_i - \overline{X} \big)^2} \quad ①
\end{cases}
$$

4. prove

- numerator

$$\begin{aligned}
\sum \big(x_i-\overline{X}\big) \big(y_i-\overline{Y}\big)
& = \sum \big(x_iy_i - x_i \overline{Y} - \overline{X}y_i + \overline{X}\overline{Y} \big) \\ \\
& = \sum x_iy_i - \sum x_i \overline{Y} - \sum \overline{X}y_i + \sum \overline{X}\overline{Y} \\ \\ 
& = \sum x_iy_i - n \overline{X} \overline{Y} - n \overline{X} \overline{Y} + n \overline{X} \overline{Y} \\ \\
& = \sum x_iy_i - \overline{Y} \sum x_i
\end{aligned}
$$

- denominator

$$
\begin{aligned}
\sum \big(x_i - \overline{X} \big)^2 & = \sum \big(x_i^2 -2x_i \overline{X} + \overline{X}^2 \big) \\ \\
& = \sum x_i^2 - 2\overline{X}\sum x_i + \sum \overline{X}^2 \\ \\
& = \sum x_i^2 - 2n\overline{X}^2 + n \overline{X}^2 \\ \\
& = \sum x_i^2 - n \overline{X}^2 \\ \\
& = \sum x_i^2 - \overline{X} \sum x_i
\end{aligned}
$$

## end